---
title: "Math Pill #2: Square Roots"
mathjax: true
tags:
  - Math
  - Learning
description: >
  Simplifying radicals is strangely satisfying. 
---

Simplifying radicals is strangely satisfying.

<p class="info-bubble" markdown="1">
I'm helping my son with mathematics, and I have to re-learn it, but this is fun. Hence, I'm hoping to start a [series of articles](/blog/tag/math/).
</p>

## Problem statement

Given:

$$
\begin{cases}
\begin{aligned}
A &= \sqrt{4 + \sqrt{11} + \sqrt{23 - 2\sqrt{132}}} \\
B &= \sqrt{\sqrt{97 + 56\sqrt{3}}}
\end{aligned}
\end{cases}
$$

Show that:

$$
\frac{B^2 - 4A}{B - A} \in \mathbb{N}.
$$

## Solution

Starting with:

$$
B = \sqrt{\sqrt{97 + 56\sqrt{3}}}
$$

Often such sums can be rewritten like this:

$$
97 + 56\sqrt{3} = (\sqrt{a} + \sqrt{b})^2
$$

We observe the formula:

$$
(\sqrt{a} + \sqrt{b})^2 = a + b + 2\sqrt{ab}
$$

Therefore, we end up with the following system of equations:

$$
\begin{cases}
a + b = 97 \\
ab = 28^2 \cdot 3
\end{cases}
$$

The solutions may or may not jump at you, but there's a little [Vieta's formula](https://en.wikipedia.org/wiki/Vieta%27s_formulas) that can help â€” we can find `a` and `b` as being the solutions to this quadratic equation:

$$
\begin{aligned}
(x - a)(x + b) &= 0 \iff \\
x^2 - (a + b)x + ab &= 0 \iff \\
x^2 - 97 x + 2352 &= 0
\end{aligned}
$$

Solving that:

$$
\begin{aligned}
\Delta &= 97^2 - 4 \cdot 2352 \\
&= 9409 - 9408 \\
&= 1 \\
x_1 &= a = \frac{97 + \sqrt{1}}{2} = 49 \\
x_2 &= b = \frac{97 - \sqrt{1}}{2} = 48
\end{aligned}
$$

Threfore:

$$
\begin{aligned}
97 + 56\sqrt{3} &= (\sqrt{49} + \sqrt{48})^2 \\
&= (7 + 4\sqrt{3})^2
\end{aligned}
$$

Going back to our original value, we rewrite it:

$$
\begin{aligned}
B &= \sqrt{\sqrt{97 + 56\sqrt{3}}} \\
&= \sqrt{\sqrt{(7 + 4\sqrt{3})^2}} \\
&= \sqrt{7 + 4\sqrt{3}}
\end{aligned}
$$

We still have a square of a sum, but this time we can spot the $(a + b)^2$ formula easily:

$$
\begin{aligned}
B &= \sqrt{7 + 4\sqrt{3}} \\
&= \sqrt{2^2 + 2 \cdot 2\sqrt{3} + \sqrt{3}^2} \\
&= \sqrt{(2 + \sqrt{3})^2} \\
&= 2 + \sqrt{3}
\end{aligned}
$$

Next, for simplifying A, we'll focus on rewriting this:

$$
23 - 2\sqrt{132} = (\sqrt{a} - \sqrt{b})^2
$$

Same trick applies, so we're dealing with this system:

$$
\begin{cases}
a + b = 23 \\
ab = 132
\end{cases}
$$

Which will have solutions generated by this quadratic equation:

$$
x^2 - 23x + 132 = 0
$$

Solving it:

$$
\begin{aligned}
\Delta &= 23^2 - 4 \cdot 132 = 529 - 528 = 1 \\
x_1 &= a = \frac{23 + 1}{2} = \frac{24}{2} = 12 \\
x_2 &= b = \frac{23 - 1}{2} = \frac{22}{2} = 11
\end{aligned}
$$

Therefore our sum can be rewritten as (we remember that we have a minus sign though ðŸ™‚):

$$
\begin{aligned}
23 - 2\sqrt{132} &= (\sqrt{12} - \sqrt{11})^2 \\
&= (2\sqrt{3} - \sqrt{11})^2
\end{aligned}
$$

We can now rewrite our A:

$$
\begin{aligned}
A &= \sqrt{4 + \sqrt{11} + \sqrt{23 - 2\sqrt{132}}} \\
  &= \sqrt{4 + \sqrt{11} + \sqrt{(2\sqrt{3} - \sqrt{11})^2}} \\
  &= \sqrt{4 + \sqrt{11} + 2\sqrt{3} - \sqrt{11}} \\
  &= \sqrt{4 + 2\sqrt{3}} \\
  &= \sqrt{1^2 + 2\sqrt{3} + \sqrt{3}^2} \\
  &= \sqrt{(1 + \sqrt{3})^2} \\
  &= 1 + \sqrt{3}
\end{aligned}
$$

And finally:

$$
\begin{aligned}
\frac{B^2 - 4A}{B - A} 
&= \frac{(2 + \sqrt{3})^2 - 4(1 + \sqrt{3})}{(2 + \sqrt{3}) - (1 + \sqrt{3})} \\
&= \frac{4 + 4\sqrt{3} + 3 - 4 - 4\sqrt{3}}{1} \\
&= 3 \in \mathbb{N}
\end{aligned}
$$
